more proofs

proof/extraction/XMSS_IMPL.ec
@@ -335,106 +335,6 @@ module M(SC:Syscall_t) = {
     return (out);
   }
   
-  proc _blocks_0_ref_96 (_H:W32.t Array8.t, in_0:W8.t Array96.t) : W32.t Array8.t *
-                                                                   W64.t = {
-    var aux: int;
-    
-    var offset:W64.t;
-    var inlen:W64.t;
-    var kp:W32.t Array64.t;
-    var hp:W32.t Array8.t;
-    var h:W32.t Array8.t;
-    var t:int;
-    var v:W32.t;
-    var w:W32.t Array64.t;
-    var a:W32.t;
-    var b:W32.t;
-    var c:W32.t;
-    var d:W32.t;
-    var e:W32.t;
-    var f:W32.t;
-    var g:W32.t;
-    var h_0:W32.t;
-    var tr:W64.t;
-    var t1:W32.t;
-    var r:W32.t;
-    var t2:W32.t;
-    h <- witness;
-    hp <- witness;
-    kp <- witness;
-    w <- witness;
-    offset <- (W64.of_int 0);
-    inlen <- (W64.of_int 96);
-    kp <- sHA256_K;
-    hp <- _H;
-    h <- hp;
-    if ((64 <= 96)) {
-      
-      while (((W64.of_int 64) \ule inlen)) {
-        (* Erased call to spill *)
-        t <- 0;
-        while (t < 16) {
-          v <-
-          (get32_direct (WArray96.init8 (fun i => (in_0).[i]))
-          (W64.to_uint (offset + (W64.of_int (4 * t)))));
-          v <- BSWAP_32 v;
-          w.[t] <- v;
-          t <- t + 1;
-        }
-        (* Erased call to spill *)
-        t <- 16;
-        while (t < 64) {
-          w <@ __Wt_ref (w, t);
-          t <- t + 1;
-        }
-        (a, b, c, d, e, f, g, h_0, h) <@ __load_H_ref (h);
-        hp <- h;
-        tr <- (W64.of_int 0);
-        
-        while ((tr \ult (W64.of_int 64))) {
-          t1 <- h_0;
-          r <@ __BSIG1_ref (e);
-          t1 <- (t1 + r);
-          r <@ __CH_ref (e, f, g);
-          t1 <- (t1 + r);
-          t1 <- (t1 + kp.[(W64.to_uint tr)]);
-          t1 <- (t1 + w.[(W64.to_uint tr)]);
-          t2 <@ __BSIG0_ref (a);
-          r <@ __MAJ_ref (a, b, c);
-          t2 <- (t2 + r);
-          h_0 <- g;
-          g <- f;
-          f <- e;
-          e <- d;
-          e <- (e + t1);
-          d <- c;
-          c <- b;
-          b <- a;
-          a <- t1;
-          a <- (a + t2);
-          tr <- (tr + (W64.of_int 1));
-        }
-        h <- hp;
-        a <- (a + h.[0]);
-        b <- (b + h.[1]);
-        c <- (c + h.[2]);
-        d <- (d + h.[3]);
-        e <- (e + h.[4]);
-        f <- (f + h.[5]);
-        g <- (g + h.[6]);
-        h_0 <- (h_0 + h.[7]);
-        h <@ __store_H_ref (h, a, b, c, d, e, f, g, h_0);
-        (* Erased call to unspill *)
-        offset <- (offset + (W64.of_int 64));
-        inlen <- (inlen - (W64.of_int 64));
-      }
-    } else {
-      
-    }
-    _H <- h;
-    return (_H, offset);
-  }
-  
   proc _blocks_0_ref_128 (_H:W32.t Array8.t, in_0:W8.t Array128.t) : 
   W32.t Array8.t * W64.t = {
     var aux: int;
@@ -535,55 +435,104 @@ module M(SC:Syscall_t) = {
     return (_H, offset);
   }
   
-  proc __lastblocks_ref_96 (in_0:W8.t Array96.t, inlen:W64.t, offset:W64.t,
-                            bits:W64.t) : W32.t Array32.t * W64.t = {
+  proc _blocks_0_ref_96 (_H:W32.t Array8.t, in_0:W8.t Array96.t) : W32.t Array8.t *
+                                                                   W64.t = {
     var aux: int;
     
-    var sblocks:W32.t Array32.t;
-    var nblocks:W64.t;
-    var i:W64.t;
-    var k:int;
-    var index:W64.t;
-    var v:W8.t;
-    var j:W64.t;
-    sblocks <- witness;
-    i <- (W64.of_int 0);
-    k <- 0;
-    while (k < 32) {
-      sblocks.[k] <- (truncateu32 i);
-      k <- k + 1;
-    }
-    
-    while ((i \ult inlen)) {
-      index <- offset;
-      index <- (index + i);
-      v <- in_0.[(W64.to_uint index)];
-      sblocks <-
-      Array32.init
-      (WArray128.get32 (WArray128.set8 (WArray128.init32 (fun i_0 => (sblocks).[i_0])) (W64.to_uint i) (v)));
-      i <- (i + (W64.of_int 1));
-    }
-    sblocks <-
-    Array32.init
-    (WArray128.get32 (WArray128.set8 (WArray128.init32 (fun i_0 => (sblocks).[i_0])) (W64.to_uint i) ((W8.of_int 128))));
-    if ((inlen \ult (W64.of_int 56))) {
-      j <- (W64.of_int (64 - 8));
-      nblocks <- (W64.of_int 1);
-      i <- (W64.of_int 63);
+    var offset:W64.t;
+    var inlen:W64.t;
+    var kp:W32.t Array64.t;
+    var hp:W32.t Array8.t;
+    var h:W32.t Array8.t;
+    var t:int;
+    var v:W32.t;
+    var w:W32.t Array64.t;
+    var a:W32.t;
+    var b:W32.t;
+    var c:W32.t;
+    var d:W32.t;
+    var e:W32.t;
+    var f:W32.t;
+    var g:W32.t;
+    var h_0:W32.t;
+    var tr:W64.t;
+    var t1:W32.t;
+    var r:W32.t;
+    var t2:W32.t;
+    h <- witness;
+    hp <- witness;
+    kp <- witness;
+    w <- witness;
+    offset <- (W64.of_int 0);
+    inlen <- (W64.of_int 96);
+    kp <- sHA256_K;
+    hp <- _H;
+    h <- hp;
+    if ((64 <= 96)) {
+      
+      while (((W64.of_int 64) \ule inlen)) {
+        (* Erased call to spill *)
+        t <- 0;
+        while (t < 16) {
+          v <-
+          (get32_direct (WArray96.init8 (fun i => (in_0).[i]))
+          (W64.to_uint (offset + (W64.of_int (4 * t)))));
+          v <- BSWAP_32 v;
+          w.[t] <- v;
+          t <- t + 1;
+        }
+        (* Erased call to spill *)
+        t <- 16;
+        while (t < 64) {
+          w <@ __Wt_ref (w, t);
+          t <- t + 1;
+        }
+        (a, b, c, d, e, f, g, h_0, h) <@ __load_H_ref (h);
+        hp <- h;
+        tr <- (W64.of_int 0);
+        
+        while ((tr \ult (W64.of_int 64))) {
+          t1 <- h_0;
+          r <@ __BSIG1_ref (e);
+          t1 <- (t1 + r);
+          r <@ __CH_ref (e, f, g);
+          t1 <- (t1 + r);
+          t1 <- (t1 + kp.[(W64.to_uint tr)]);
+          t1 <- (t1 + w.[(W64.to_uint tr)]);
+          t2 <@ __BSIG0_ref (a);
+          r <@ __MAJ_ref (a, b, c);
+          t2 <- (t2 + r);
+          h_0 <- g;
+          g <- f;
+          f <- e;
+          e <- d;
+          e <- (e + t1);
+          d <- c;
+          c <- b;
+          b <- a;
+          a <- t1;
+          a <- (a + t2);
+          tr <- (tr + (W64.of_int 1));
+        }
+        h <- hp;
+        a <- (a + h.[0]);
+        b <- (b + h.[1]);
+        c <- (c + h.[2]);
+        d <- (d + h.[3]);
+        e <- (e + h.[4]);
+        f <- (f + h.[5]);
+        g <- (g + h.[6]);
+        h_0 <- (h_0 + h.[7]);
+        h <@ __store_H_ref (h, a, b, c, d, e, f, g, h_0);
+        (* Erased call to unspill *)
+        offset <- (offset + (W64.of_int 64));
+        inlen <- (inlen - (W64.of_int 64));
+      }
     } else {
-      j <- (W64.of_int (128 - 8));
-      nblocks <- (W64.of_int 2);
-      i <- (W64.of_int 127);
+      
     }
-    
-    while ((j \ule i)) {
-      sblocks <-
-      Array32.init
-      (WArray128.get32 (WArray128.set8 (WArray128.init32 (fun i_0 => (sblocks).[i_0])) (W64.to_uint i) ((truncateu8 bits))));
-      bits <- (bits `>>` (W8.of_int 8));
-      i <- (i - (W64.of_int 1));
-    }
-    return (sblocks, nblocks);
+    _H <- h;
+    return (_H, offset);
   }
   
   proc __lastblocks_ref_128 (in_0:W8.t Array128.t, inlen:W64.t, offset:W64.t,
@@ -637,39 +586,55 @@ module M(SC:Syscall_t) = {
     return (sblocks, nblocks);
   }
   
-  proc __sha256_96 (out:W8.t Array32.t, in_0:W8.t Array96.t) : W8.t Array32.t = {
+  proc __lastblocks_ref_96 (in_0:W8.t Array96.t, inlen:W64.t, offset:W64.t,
+                            bits:W64.t) : W32.t Array32.t * W64.t = {
+    var aux: int;
     
-    var bits:W64.t;
-    var h:W32.t Array8.t;
-    var hp:W32.t Array8.t;
-    var offset:W64.t;
-    var inlen:W64.t;
     var sblocks:W32.t Array32.t;
     var nblocks:W64.t;
-    var sblocksp:W32.t Array32.t;
-    var  _0:W32.t Array32.t;
-     _0 <- witness;
-    h <- witness;
-    hp <- witness;
+    var i:W64.t;
+    var k:int;
+    var index:W64.t;
+    var v:W8.t;
+    var j:W64.t;
     sblocks <- witness;
-    sblocksp <- witness;
-    (* Erased call to spill *)
-    bits <- (W64.of_int 96);
-    bits <- (bits `<<` (W8.of_int 3));
-    (* Erased call to spill *)
-    h <@ __initH_ref ();
-    (* Erased call to spill *)
-    hp <- h;
-    (hp, offset) <@ _blocks_0_ref_96 (hp, in_0);
-    (* Erased call to unspill *)
-    inlen <- (W64.of_int (96 %% 64));
-    (sblocks, nblocks) <@ __lastblocks_ref_96 (in_0, inlen, offset, bits);
-    sblocksp <- sblocks;
-    (hp,  _0) <@ _blocks_1_ref (hp, sblocksp, nblocks);
-    (* Erased call to unspill *)
-    h <- hp;
-    out <@ __store_ref_array (out, h);
-    return (out);
+    i <- (W64.of_int 0);
+    k <- 0;
+    while (k < 32) {
+      sblocks.[k] <- (truncateu32 i);
+      k <- k + 1;
+    }
+    
+    while ((i \ult inlen)) {
+      index <- offset;
+      index <- (index + i);
+      v <- in_0.[(W64.to_uint index)];
+      sblocks <-
+      Array32.init
+      (WArray128.get32 (WArray128.set8 (WArray128.init32 (fun i_0 => (sblocks).[i_0])) (W64.to_uint i) (v)));
+      i <- (i + (W64.of_int 1));
+    }
+    sblocks <-
+    Array32.init
+    (WArray128.get32 (WArray128.set8 (WArray128.init32 (fun i_0 => (sblocks).[i_0])) (W64.to_uint i) ((W8.of_int 128))));
+    if ((inlen \ult (W64.of_int 56))) {
+      j <- (W64.of_int (64 - 8));
+      nblocks <- (W64.of_int 1);
+      i <- (W64.of_int 63);
+    } else {
+      j <- (W64.of_int (128 - 8));
+      nblocks <- (W64.of_int 2);
+      i <- (W64.of_int 127);
+    }
+    
+    while ((j \ule i)) {
+      sblocks <-
+      Array32.init
+      (WArray128.get32 (WArray128.set8 (WArray128.init32 (fun i_0 => (sblocks).[i_0])) (W64.to_uint i) ((truncateu8 bits))));
+      bits <- (bits `>>` (W8.of_int 8));
+      i <- (i - (W64.of_int 1));
+    }
+    return (sblocks, nblocks);
   }
   
   proc __sha256_128 (out:W8.t Array32.t, in_0:W8.t Array128.t) : W8.t Array32.t = {
@@ -699,6 +664,41 @@ module M(SC:Syscall_t) = {
     (* Erased call to unspill *)
     inlen <- (W64.of_int (128 %% 64));
     (sblocks, nblocks) <@ __lastblocks_ref_128 (in_0, inlen, offset, bits);
+    sblocksp <- sblocks;
+    (hp,  _0) <@ _blocks_1_ref (hp, sblocksp, nblocks);
+    (* Erased call to unspill *)
+    h <- hp;
+    out <@ __store_ref_array (out, h);
+    return (out);
+  }
+  
+  proc __sha256_96 (out:W8.t Array32.t, in_0:W8.t Array96.t) : W8.t Array32.t = {
+    
+    var bits:W64.t;
+    var h:W32.t Array8.t;
+    var hp:W32.t Array8.t;
+    var offset:W64.t;
+    var inlen:W64.t;
+    var sblocks:W32.t Array32.t;
+    var nblocks:W64.t;
+    var sblocksp:W32.t Array32.t;
+    var  _0:W32.t Array32.t;
+     _0 <- witness;
+    h <- witness;
+    hp <- witness;
+    sblocks <- witness;
+    sblocksp <- witness;
+    (* Erased call to spill *)
+    bits <- (W64.of_int 96);
+    bits <- (bits `<<` (W8.of_int 3));
+    (* Erased call to spill *)
+    h <@ __initH_ref ();
+    (* Erased call to spill *)
+    hp <- h;
+    (hp, offset) <@ _blocks_0_ref_96 (hp, in_0);
+    (* Erased call to unspill *)
+    inlen <- (W64.of_int (96 %% 64));
+    (sblocks, nblocks) <@ __lastblocks_ref_96 (in_0, inlen, offset, bits);
     sblocksp <- sblocks;
     (hp,  _0) <@ _blocks_1_ref (hp, sblocksp, nblocks);
     (* Erased call to unspill *)
@@ -961,21 +961,6 @@ module M(SC:Syscall_t) = {
     return (out);
   }
   
-  proc __ull_to_bytes_4 (out:W8.t Array4.t, in_0:W64.t) : W8.t Array4.t = {
-    var aux: int;
-    
-    var i:int;
-    
-    aux <- (- 1);
-    i <- (4 - 1);
-    while (aux < i) {
-      out.[i] <- (truncateu8 in_0);
-      in_0 <- (in_0 `>>` (W8.of_int 8));
-      i <- i - 1;
-    }
-    return (out);
-  }
-  
   proc __ull_to_bytes_32 (out:W8.t Array32.t, in_0:W64.t) : W8.t Array32.t = {
     var aux: int;
     
@@ -998,6 +983,21 @@ module M(SC:Syscall_t) = {
     
     aux <- (- 1);
     i <- (2 - 1);
+    while (aux < i) {
+      out.[i] <- (truncateu8 in_0);
+      in_0 <- (in_0 `>>` (W8.of_int 8));
+      i <- i - 1;
+    }
+    return (out);
+  }
+  
+  proc __ull_to_bytes_4 (out:W8.t Array4.t, in_0:W64.t) : W8.t Array4.t = {
+    var aux: int;
+    
+    var i:int;
+    
+    aux <- (- 1);
+    i <- (4 - 1);
     while (aux < i) {
       out.[i] <- (truncateu8 in_0);
       in_0 <- (in_0 `>>` (W8.of_int 8));
@@ -1034,7 +1034,7 @@ module M(SC:Syscall_t) = {
     return (result);
   }
   
-  proc __bytes_to_ull_ptr (in_ptr:W64.t, inlen:W64.t) : W64.t = {
+  proc __bytes_to_ull_ptr (in_ptr:W64.t) : W64.t = {
     
     var result:W64.t;
     var i:W64.t;
@@ -1050,10 +1050,9 @@ module M(SC:Syscall_t) = {
     result <- (W64.of_int 0);
     i <- (W64.of_int 0);
     
-    while ((i \ult inlen)) {
+    while ((i \ult (W64.of_int 4))) {
       t <- (zeroextu64 (loadW8 Glob.mem (W64.to_uint (in_ptr + i))));
-      u <- inlen;
-      u <- (u - (W64.of_int 1));
+      u <- (W64.of_int (4 - 1));
       u <- (u - i);
       (_of_, _cf_, _sf_,  _0, _zf_, u) <- SHL_64 u (W8.of_int 3);
       (_of_, _cf_, _sf_,  _1, _zf_, t) <- SHL_64 t (truncateu8 u);
@@ -1103,19 +1102,6 @@ module M(SC:Syscall_t) = {
     return (a);
   }
   
-  proc __memset_u8_128 (a:W8.t Array128.t, value:W8.t) : W8.t Array128.t = {
-    
-    var i:W64.t;
-    
-    i <- (W64.of_int 0);
-    
-    while ((i \ult (W64.of_int 128))) {
-      a.[(W64.to_uint i)] <- value;
-      i <- (i + (W64.of_int 1));
-    }
-    return (a);
-  }
-  
   proc __memset_u8_4 (a:W8.t Array4.t, value:W8.t) : W8.t Array4.t = {
     
     var i:W64.t;
@@ -1123,6 +1109,19 @@ module M(SC:Syscall_t) = {
     i <- (W64.of_int 0);
     
     while ((i \ult (W64.of_int 4))) {
+      a.[(W64.to_uint i)] <- value;
+      i <- (i + (W64.of_int 1));
+    }
+    return (a);
+  }
+  
+  proc __memset_u8_128 (a:W8.t Array128.t, value:W8.t) : W8.t Array128.t = {
+    
+    var i:W64.t;
+    
+    i <- (W64.of_int 0);
+    
+    while ((i \ult (W64.of_int 128))) {
       a.[(W64.to_uint i)] <- value;
       i <- (i + (W64.of_int 1));
     }
@@ -1161,8 +1160,8 @@ module M(SC:Syscall_t) = {
     return (out);
   }
   
-  proc __memcpy_u8u8_64_32 (out:W8.t Array64.t, in_0:W8.t Array32.t) : 
-  W8.t Array64.t = {
+  proc __memcpy_u8u8_32_32 (out:W8.t Array32.t, in_0:W8.t Array32.t) : 
+  W8.t Array32.t = {
     
     var i:W64.t;
     
@@ -1189,8 +1188,8 @@ module M(SC:Syscall_t) = {
     return (out);
   }
   
-  proc __memcpy_u8u8_32_32 (out:W8.t Array32.t, in_0:W8.t Array32.t) : 
-  W8.t Array32.t = {
+  proc __memcpy_u8u8_64_32 (out:W8.t Array64.t, in_0:W8.t Array32.t) : 
+  W8.t Array64.t = {
     
     var i:W64.t;
     
@@ -1203,12 +1202,12 @@ module M(SC:Syscall_t) = {
     return (out);
   }
   
-  proc _memcpy_u8u8_64_32 (out:W8.t Array64.t, in_0:W8.t Array32.t) : 
-  W8.t Array64.t = {
+  proc _memcpy_u8u8_32_32 (out:W8.t Array32.t, in_0:W8.t Array32.t) : 
+  W8.t Array32.t = {
     
     
     
-    out <@ __memcpy_u8u8_64_32 (out, in_0);
+    out <@ __memcpy_u8u8_32_32 (out, in_0);
     return (out);
   }
   
@@ -1221,23 +1220,23 @@ module M(SC:Syscall_t) = {
     return (out);
   }
   
-  proc _memcpy_u8u8_32_32 (out:W8.t Array32.t, in_0:W8.t Array32.t) : 
-  W8.t Array32.t = {
+  proc _memcpy_u8u8_64_32 (out:W8.t Array64.t, in_0:W8.t Array32.t) : 
+  W8.t Array64.t = {
     
     
     
-    out <@ __memcpy_u8u8_32_32 (out, in_0);
+    out <@ __memcpy_u8u8_64_32 (out, in_0);
     return (out);
   }
   
-  proc _x_memcpy_u8u8_64_32 (out:W8.t Array64.t, in_0:W8.t Array32.t) : 
-  W8.t Array64.t = {
+  proc _x_memcpy_u8u8_32_32 (out:W8.t Array32.t, in_0:W8.t Array32.t) : 
+  W8.t Array32.t = {
     
     
     
     out <- out;
     in_0 <- in_0;
-    out <@ _memcpy_u8u8_64_32 (out, in_0);
+    out <@ _memcpy_u8u8_32_32 (out, in_0);
     out <- out;
     return (out);
   }
@@ -1254,14 +1253,14 @@ module M(SC:Syscall_t) = {
     return (out);
   }
   
-  proc _x_memcpy_u8u8_32_32 (out:W8.t Array32.t, in_0:W8.t Array32.t) : 
-  W8.t Array32.t = {
+  proc _x_memcpy_u8u8_64_32 (out:W8.t Array64.t, in_0:W8.t Array32.t) : 
+  W8.t Array64.t = {
     
     
     
     out <- out;
     in_0 <- in_0;
-    out <@ _memcpy_u8u8_32_32 (out, in_0);
+    out <@ _memcpy_u8u8_64_32 (out, in_0);
     out <- out;
     return (out);
   }
@@ -1298,22 +1297,6 @@ module M(SC:Syscall_t) = {
     return (out);
   }
   
-  proc __memcpy_u8u8_2_32_2144 (out:W8.t Array32.t, in_0:W8.t Array2144.t,
-                                in_offset:W64.t, bytes:W64.t) : W8.t Array32.t *
-                                                                W64.t = {
-    
-    var i:W64.t;
-    
-    i <- (W64.of_int 0);
-    
-    while ((i \ult bytes)) {
-      out.[(W64.to_uint i)] <- in_0.[(W64.to_uint in_offset)];
-      i <- (i + (W64.of_int 1));
-      in_offset <- (in_offset + (W64.of_int 1));
-    }
-    return (out, in_offset);
-  }
-  
   proc __memcpy_u8u8_2_64_2144 (out:W8.t Array64.t, in_0:W8.t Array2144.t,
                                 in_offset:W64.t, bytes:W64.t) : W8.t Array64.t *
                                                                 W64.t = {
@@ -1330,8 +1313,24 @@ module M(SC:Syscall_t) = {
     return (out, in_offset);
   }
   
+  proc __memcpy_u8u8_2_32_2144 (out:W8.t Array32.t, in_0:W8.t Array2144.t,
+                                in_offset:W64.t, bytes:W64.t) : W8.t Array32.t *
+                                                                W64.t = {
+    
+    var i:W64.t;
+    
+    i <- (W64.of_int 0);
+    
+    while ((i \ult bytes)) {
+      out.[(W64.to_uint i)] <- in_0.[(W64.to_uint in_offset)];
+      i <- (i + (W64.of_int 1));
+      in_offset <- (in_offset + (W64.of_int 1));
+    }
+    return (out, in_offset);
+  }
+  
   proc __memcpy_u8pu8p (out_ptr:W64.t, out_offset:W64.t, in_ptr:W64.t,
-                        in_offset:W64.t, bytes:W64.t) : W64.t * W64.t * W64.t = {
+                        in_offset:W64.t, bytes:W64.t) : unit = {
     
     var i:W64.t;
     
@@ -1344,22 +1343,20 @@ module M(SC:Syscall_t) = {
       in_offset <- (in_offset + (W64.of_int 1));
       out_offset <- (out_offset + (W64.of_int 1));
     }
-    return (out_ptr, out_offset, in_offset);
+    return ();
   }
   
   proc _memcpy_u8pu8p (out_ptr:W64.t, out_offset:W64.t, in_ptr:W64.t,
-                       in_offset:W64.t, bytes:W64.t) : W64.t * W64.t * W64.t = {
+                       in_offset:W64.t, bytes:W64.t) : unit = {
     
     
     
-    (out_ptr, out_offset, in_offset) <@ __memcpy_u8pu8p (out_ptr, out_offset,
-    in_ptr, in_offset, bytes);
-    return (out_ptr, out_offset, in_offset);
+    __memcpy_u8pu8p (out_ptr, out_offset, in_ptr, in_offset, bytes);
+    return ();
   }
   
   proc _x__memcpy_u8pu8p (out_ptr:W64.t, out_offset:W64.t, in_ptr:W64.t,
-                          in_offset:W64.t, bytes:W64.t) : W64.t * W64.t *
-                                                          W64.t = {
+                          in_offset:W64.t, bytes:W64.t) : unit = {
     
     
     
@@ -1368,12 +1365,8 @@ module M(SC:Syscall_t) = {
     in_ptr <- in_ptr;
     in_offset <- in_offset;
     bytes <- bytes;
-    (out_ptr, out_offset, in_offset) <@ _memcpy_u8pu8p (out_ptr, out_offset,
-    in_ptr, in_offset, bytes);
-    out_ptr <- out_ptr;
-    out_offset <- out_offset;
-    in_offset <- in_offset;
-    return (out_ptr, out_offset, in_offset);
+    _memcpy_u8pu8p (out_ptr, out_offset, in_ptr, in_offset, bytes);
+    return ();
   }
   
   proc __memcpy_u8pu8_32 (out:W64.t, offset:W64.t, in_0:W8.t Array32.t) : 
@@ -2070,6 +2063,40 @@ module M(SC:Syscall_t) = {
     return (out, addr);
   }
   
+  proc __base_w_3_2 (output:W32.t Array3.t, input:W8.t Array2.t) : W32.t Array3.t = {
+    
+    var in_0:W64.t;
+    var bits:W64.t;
+    var total:W32.t;
+    var i:W64.t;
+    var _of_:bool;
+    var _cf_:bool;
+    var _sf_:bool;
+    var _zf_:bool;
+    var  _0:bool;
+    
+    in_0 <- (W64.of_int 0);
+    bits <- (W64.of_int 0);
+    total <- (W32.of_int 0);
+    i <- (W64.of_int 0);
+    
+    while ((i \ult (W64.of_int 3))) {
+      if ((bits = (W64.of_int 0))) {
+        total <- (zeroextu32 input.[(W64.to_uint in_0)]);
+        in_0 <- (in_0 + (W64.of_int 1));
+        bits <- (bits + (W64.of_int 8));
+      } else {
+        
+      }
+      bits <- (bits - (W64.of_int 4));
+      (_of_, _cf_, _sf_,  _0, _zf_, total) <- SHR_32 total (truncateu8 bits);
+      total <- (total `&` (W32.of_int (16 - 1)));
+      output.[(W64.to_uint i)] <- total;
+      i <- (i + (W64.of_int 1));
+    }
+    return (output);
+  }
+  
   proc __base_w_67_32 (output:W32.t Array67.t, input:W8.t Array32.t) : 
   W32.t Array67.t = {
     
@@ -2089,40 +2116,6 @@ module M(SC:Syscall_t) = {
     i <- (W64.of_int 0);
     
     while ((i \ult (W64.of_int 67))) {
-      if ((bits = (W64.of_int 0))) {
-        total <- (zeroextu32 input.[(W64.to_uint in_0)]);
-        in_0 <- (in_0 + (W64.of_int 1));
-        bits <- (bits + (W64.of_int 8));
-      } else {
-        
-      }
-      bits <- (bits - (W64.of_int 4));
-      (_of_, _cf_, _sf_,  _0, _zf_, total) <- SHR_32 total (truncateu8 bits);
-      total <- (total `&` (W32.of_int (16 - 1)));
-      output.[(W64.to_uint i)] <- total;
-      i <- (i + (W64.of_int 1));
-    }
-    return (output);
-  }
-  
-  proc __base_w_3_2 (output:W32.t Array3.t, input:W8.t Array2.t) : W32.t Array3.t = {
-    
-    var in_0:W64.t;
-    var bits:W64.t;
-    var total:W32.t;
-    var i:W64.t;
-    var _of_:bool;
-    var _cf_:bool;
-    var _sf_:bool;
-    var _zf_:bool;
-    var  _0:bool;
-    
-    in_0 <- (W64.of_int 0);
-    bits <- (W64.of_int 0);
-    total <- (W32.of_int 0);
-    i <- (W64.of_int 0);
-    
-    while ((i \ult (W64.of_int 3))) {
       if ((bits = (W64.of_int 0))) {
         total <- (zeroextu32 input.[(W64.to_uint in_0)]);
         in_0 <- (in_0 + (W64.of_int 1));
@@ -2393,25 +2386,6 @@ module M(SC:Syscall_t) = {
     }
     (_of_, _cf_, _sf_,  _0, zf,  _1) <- AND_8 acc acc;
     r <- (zf ? are_equal : r);
-    return (r);
-  }
-  
-  proc _memcmp (a:W8.t Array32.t, b:W8.t Array32.t) : W64.t = {
-    
-    var r:W64.t;
-    
-    r <@ __memcmp (a, b);
-    return (r);
-  }
-  
-  proc __memcmp_ (a:W8.t Array32.t, b:W8.t Array32.t) : W64.t = {
-    
-    var r:W64.t;
-    
-    a <- a;
-    b <- b;
-    r <@ _memcmp (a, b);
-    r <- r;
     return (r);
   }
   
@@ -2743,6 +2717,28 @@ module M(SC:Syscall_t) = {
     return (leaf, ltree_addr, ots_addr);
   }
   
+  proc __set_result (are_equal:W64.t, m_ptr:W64.t, mlen_ptr:W64.t,
+                     sm_ptr:W64.t, sm_offset:W64.t) : W64.t = {
+    
+    var res_0:W64.t;
+    var bytes:W64.t;
+    var offset_in:W64.t;
+    
+    if ((are_equal <> (W64.of_int 0))) {
+      res_0 <- (W64.of_int (- 1));
+      bytes <- (loadW64 Glob.mem (W64.to_uint (mlen_ptr + (W64.of_int 0))));
+      __memset_u8_ptr (m_ptr, bytes, (W8.of_int 0));
+      Glob.mem <-
+      storeW64 Glob.mem (W64.to_uint (mlen_ptr + (W64.of_int 0))) ((W64.of_int 0));
+    } else {
+      res_0 <- (W64.of_int 0);
+      bytes <- (loadW64 Glob.mem (W64.to_uint (mlen_ptr + (W64.of_int 0))));
+      offset_in <- sm_offset;
+      _x__memcpy_u8pu8p (m_ptr, (W64.of_int 0), sm_ptr, offset_in, bytes);
+    }
+    return (res_0);
+  }
+  
   proc __xmssmt_core_sign_open (m_ptr:W64.t, mlen_ptr:W64.t, sm_ptr:W64.t,
                                 smlen:W64.t, pk:W8.t Array64.t) : W64.t = {
     
@@ -2770,13 +2766,7 @@ module M(SC:Syscall_t) = {
     var wots_pk:W8.t Array2144.t;
     var leaf:W8.t Array32.t;
     var are_equal:W64.t;
-    var  _0:W64.t;
-    var  _1:W64.t;
-    var  _2:W64.t;
-    var  _3:bool;
-    var  _4:W64.t;
-    var  _5:W64.t;
-    var  _6:W64.t;
+    var  _0:bool;
     buf <- witness;
     leaf <- witness;
     ltree_addr <- witness;
@@ -2801,13 +2791,12 @@ module M(SC:Syscall_t) = {
     t64 <- (t64 - (W64.of_int 2500));
     Glob.mem <-
     storeW64 Glob.mem (W64.to_uint (mlen_ptr + (W64.of_int 0))) (t64);
-    idx <@ __bytes_to_ull_ptr (sm_ptr, (W64.of_int 4));
+    idx <@ __bytes_to_ull_ptr (sm_ptr);
     (* Erased call to spill *)
     offset_out <- (W64.of_int 2500);
     offset_in <- (W64.of_int 2500);
     bytes <- (loadW64 Glob.mem (W64.to_uint (mlen_ptr + (W64.of_int 0))));
-    ( _0,  _1,  _2) <@ _x__memcpy_u8pu8p (m_ptr, offset_out, sm_ptr,
-    offset_in, bytes);
+    _x__memcpy_u8pu8p (m_ptr, offset_out, sm_ptr, offset_in, bytes);
     t64 <- sm_ptr;
     t64 <- (t64 + (W64.of_int 4));
     buf <@ _x_memcpy_u8u8p_32 (buf, t64);
@@ -2826,7 +2815,7 @@ module M(SC:Syscall_t) = {
       (* Erased call to unspill *)
       idx_leaf <- (W32.of_int ((1 `<<` 10) - 1));
       idx_leaf <- (idx_leaf `&` (truncateu32 idx));
-      (_of_, _cf_, _sf_,  _3, _zf_, idx) <- SHR_64 idx (W8.of_int 10);
+      (_of_, _cf_, _sf_,  _0, _zf_, idx) <- SHR_64 idx (W8.of_int 10);
       (* Erased call to spill *)
       ots_addr <@ __set_layer_addr (ots_addr, i);
       ltree_addr <@ __set_layer_addr (ltree_addr, i);
@@ -2863,22 +2852,9 @@ module M(SC:Syscall_t) = {
       i <- (i + (W32.of_int 1));
     }
     (* Erased call to unspill *)
-    are_equal <@ __memcmp_ (root, pub_root);
-    if ((are_equal <> (W64.of_int 0))) {
-      res_0 <- (W64.of_int (- 1));
-      (* Erased call to unspill *)
-      bytes <- (loadW64 Glob.mem (W64.to_uint (mlen_ptr + (W64.of_int 0))));
-      __memset_u8_ptr (m_ptr, bytes, (W8.of_int 0));
-      Glob.mem <-
-      storeW64 Glob.mem (W64.to_uint (mlen_ptr + (W64.of_int 0))) ((W64.of_int 0));
-    } else {
-      res_0 <- (W64.of_int 0);
-      (* Erased call to unspill *)
-      bytes <- (loadW64 Glob.mem (W64.to_uint (mlen_ptr + (W64.of_int 0))));
-      offset_in <- sm_offset;
-      ( _4,  _5,  _6) <@ _x__memcpy_u8pu8p (m_ptr, (W64.of_int 0), sm_ptr,
-      offset_in, bytes);
-    }
+    are_equal <@ __memcmp (root, pub_root);
+    (* Erased call to unspill *)
+    res_0 <@ __set_result (are_equal, m_ptr, mlen_ptr, sm_ptr, sm_offset);
     return (res_0);
   }
   
@@ -3179,7 +3155,7 @@ module M(SC:Syscall_t) = {
     seed_p <- witness;
     seed_p <- seed;
     seed_p <@ SC.randombytes_96 (seed_p);
-    (pk, sk) <@ __xmssmt_core_seed_keypair (pk, sk, seed);
+    (pk, sk) <@ __xmssmt_core_seed_keypair (pk, sk, seed_p);
     return (pk, sk);
   }
   
@@ -3236,10 +3212,7 @@ module M(SC:Syscall_t) = {
     var auth_path:W8.t Array320.t;
     var  _0:W64.t;
     var  _1:W64.t;
-    var  _2:W64.t;
-    var  _3:W64.t;
-    var  _4:W64.t;
-    var  _5:bool;
+    var  _2:bool;
     auth_path <- witness;
     buf <- witness;
     idx_bytes <- witness;
@@ -3253,8 +3226,8 @@ module M(SC:Syscall_t) = {
     (* Erased call to spill *)
     ots_addr <@ __zero_address_ (ots_addr);
     ots_addr <@ __set_type (ots_addr, (W32.of_int 0));
-    ( _0,  _1,  _2) <@ _x__memcpy_u8pu8p (sm_ptr, (W64.of_int 2500), m_ptr,
-    (W64.of_int 0), mlen);
+    _x__memcpy_u8pu8p (sm_ptr, (W64.of_int 2500), m_ptr, (W64.of_int 0),
+    mlen);
     t64 <- mlen;
     t64 <- (t64 + (W64.of_int 2500));
     Glob.mem <-
@@ -3287,7 +3260,7 @@ module M(SC:Syscall_t) = {
       
     }
     if ((exit_0 <> (W8.of_int 1))) {
-      (sm_ptr,  _3) <@ _x_memcpy_u8pu8_4 (sm_ptr, (W64.of_int 0),
+      (sm_ptr,  _0) <@ _x_memcpy_u8pu8_4 (sm_ptr, (W64.of_int 0),
       (Array4.init (fun i_0 => sk.[0 + i_0])));
       (* Erased call to unspill *)
       t64 <- idx;
@@ -3299,7 +3272,7 @@ module M(SC:Syscall_t) = {
       idx_bytes <@ __ull_to_bytes_32 (idx_bytes, idx);
       sk_prf <- (Array32.init (fun i_0 => sk.[(4 + 32) + i_0]));
       buf <@ __prf_ (buf, idx_bytes, sk_prf);
-      (sm_ptr,  _4) <@ _x_memcpy_u8pu8_32 (sm_ptr, (W64.of_int 4), buf);
+      (sm_ptr,  _1) <@ _x_memcpy_u8pu8_32 (sm_ptr, (W64.of_int 4), buf);
       (* Erased call to unspill *)
       pub_root <- (Array32.init (fun i_0 => sk.[(4 + (2 * 32)) + i_0]));
       j <- 0;
@@ -3326,7 +3299,7 @@ module M(SC:Syscall_t) = {
         (* Erased call to unspill *)
         idx_leaf <- (W32.of_int ((1 `<<` 10) - 1));
         idx_leaf <- (idx_leaf `&` (truncateu32 idx));
-        (_of_, _cf_, _sf_,  _5, _zf_, idx) <- SHR_64 idx (W8.of_int 10);
+        (_of_, _cf_, _sf_,  _2, _zf_, idx) <- SHR_64 idx (W8.of_int 10);
         (* Erased call to spill *)
         ots_addr <@ __set_layer_addr (ots_addr, i);
         ots_addr <@ __set_tree_addr (ots_addr, idx);
