proof/correctness/Termination.ec
@@ -5,6 +5,26 @@ require import XMSS_IMPL XMSS_IMPL_PP Generic Parameters.
 
 from Jasmin require import JModel.
 
+lemma bytes_to_ull_ptr_ll : islossless Mp(Syscall).__bytes_to_ull_ptr.
+proof.
+proc.
+while (0 <= to_uint i <= 4) (4 - to_uint i) ; auto => /> * ; last by smt(@W64).
+do split.
+  + rewrite to_uintD /#.
+  + smt(@W64).
+  + rewrite to_uintD ; smt(@W64).
+qed.
+
+lemma bytes_to_ull_ll : islossless Mp(Syscall).__bytes_to_ull.
+proof.
+proc.
+while (0 <= to_uint i <= 4) (4 - to_uint i); auto => /> *; last by smt(@W64).
+do split.
+  + rewrite to_uintD /#.
+  + smt(@W64).
+  + rewrite to_uintD ; smt(@W64).
+qed.
+
 lemma ull_to_bytes_2_ll  : islossless Mp(Syscall).__ull_to_bytes_2 
     by proc ; while (true) (i - aux) ; by auto => /> /#.
 
@@ -29,6 +49,28 @@ while (0 <= to_uint i <= 32) (32 - to_uint i) ; auto => /> *.
 - smt(@W64).
 qed.
 
+lemma memcpy_32_ptr_ll : islossless Mp(Syscall).__memcpy_u8pu8_32.
+proof.
+proc.
+while (0 <= to_uint i <= 32) (32 - to_uint i) ; auto => /> *.
+- do split.
+  + rewrite to_uintD_small /#.
+  + smt(@W64).
+  + rewrite to_uintD ; smt(@W64).
+- smt(@W64).
+qed.
+
+lemma memcpy_ptr_ptr_ll : islossless Mp(Syscall).__memcpy_u8pu8p.
+proof.
+proc.
+while (0 <= to_uint i <= to_uint bytes) ((to_uint bytes) - (to_uint i)) ; auto => /> *.
+- do split.
+  + rewrite to_uintD ; smt(@W64).
+  + smt(@W64).
+  + smt(@W64).
+- smt(@W64).
+qed.
+
 lemma memset_zero_ll : islossless Mp(Syscall).__memset_zero_u8.
 proof.
 proc.
@@ -40,29 +82,69 @@ do split.
 - smt(@W64).
 qed.
 
+lemma memset_u8_ptr_ll : phoare [Mp(Syscall).__memset_u8_ptr : 0 <= to_uint inlen < W64.modulus ==> true] = 1%r.
+proof.
+proc.
+while (0 <= to_uint i <= to_uint inlen) ((to_uint inlen) - (to_uint i)) ; auto => /> ; progress ; smt(@W64).
+qed.
+
+lemma memset_4_ll : islossless Mp(Syscall).__memset_u8_4.
+proof.
+proc.
+while (0 <= to_uint i <= 4) (4 - to_uint i); auto => /> *; last by smt(@W64).
+do split ; [rewrite to_uintD /# | smt(@W64) | rewrite to_uintD ; smt(@W64)].
+qed.
+
+lemma memset_128_ll : islossless Mp(Syscall).__memset_u8_128.
+proof.
+proc.
+while (0 <= to_uint i <= 128) (128 - to_uint i); auto => /> *; last by smt(@W64).
+do split ; [rewrite to_uintD /# | smt(@W64) | rewrite to_uintD ; smt(@W64)].
+qed.
+
+lemma memcmp_ll : islossless Mp(Syscall).__memcmp.
+proof.
+proc.
+sp ; wp.
+while (0 <= to_uint i <= 32) (32 - to_uint i) ; auto => />.
+- progress.
+  + rewrite to_uintD_small /#.
+  + smt(@W64).
+  + rewrite to_uintD ; smt(@W64).
+- progress ; smt(@W64).
+qed.
+
 lemma thash_f_ll : islossless Mp(Syscall).__thash_f.
 proof.
 proc.
 auto => />.
 while (0 <= to_uint i <= 32) (32 - to_uint i) ; auto => />.
-  - auto => /> &hr *. do split ; 1,2: by smt(@W64). rewrite to_uintD_small => /#.
+  - auto => /> *. do split ; 1,2: by smt(@W64). rewrite to_uintD_small => /#.
   - auto => /> *. split ; [ progress ; rewrite ultE => /# | auto ].
-  - call (addr_to_bytes_ll). inline Mp(Syscall).__set_key_and_mask ; auto => />. 
-    call (addr_to_bytes_ll) ; auto => />. 
-    call (ull_to_bytes_32_ll). auto => /> *. rewrite ultE => /#.
+  - call addr_to_bytes_ll. inline Mp(Syscall).__set_key_and_mask ; auto => />. 
+    call addr_to_bytes_ll ; auto => />. 
+    call ull_to_bytes_32_ll. auto => /> *. rewrite ultE => /#.
 qed.
 
 lemma thash_h_ll : islossless Mp(Syscall).__thash_h.
 proof.
 proc.
-inline  Mp(Syscall).__set_key_and_mask.
-wp.
+inline  Mp(Syscall).__set_key_and_mask ; wp.
 while (0 <= to_uint i <= 2 * 32) ((2*32) - (to_uint i)).
 - auto => />. progress.
   + rewrite to_uintD_small /#.
   + smt(@W64).
   + rewrite to_uintD_small ; [smt() | smt(@W64)].
 - wp. do (call addr_to_bytes_ll ; wp). call ull_to_bytes_32_ll. auto => /> *. smt(@W64).
+qed.
+
+lemma hash_msg_ll : islossless Mp(Syscall).__hash_message.
+proof.
+proc.
+inline Mp(Syscall)._x_memcpy_u8pu8_32 Mp(Syscall)._memcpy_u8pu8_32 ; wp.
+call memcpy_32_ptr_ll ; wp. call ull_to_bytes_32_ll ; wp.
+do (call memcpy_32_ptr_ll ; wp). call ull_to_bytes_32_ll ; wp.
+by skip.
 qed.
 
 lemma base_w_ll : phoare [BaseWGeneric.__base_w : size output <= 67 ==> true] = 1%r.
@@ -89,7 +171,7 @@ lemma csum_ll : islossless Mp(Syscall).__csum.
 proof.
 proc.
 while (0 <= to_uint i <= 64) (64 - to_uint i); auto => />.
-  - move => &hr. rewrite ultE of_uintK /= => *. rewrite to_uintD_small => /#.
+  - move => ?. rewrite ultE of_uintK /= => *. rewrite to_uintD_small => /#.
   - move => ?. rewrite ultE => /= /#. 
 qed.
 
@@ -105,7 +187,6 @@ auto => /> *.
 by rewrite /to_list size_mkseq.
 qed.
 
-(* Gen Chain *)
 lemma gen_chain_inplace_ll : phoare[Mp(Syscall).__gen_chain_inplace : 
     0 <= to_uint steps <= XMSS_WOTS_W ==> true] = 1%r.
 proof.
@@ -127,16 +208,16 @@ while (#pre /\ 0 <= to_uint i <= to_uint (start + steps) /\ t = start + steps)
       ((to_uint t) - (to_uint i)) ; auto => /> ; 2: by smt(@W32).
 - inline Mp(Syscall).__set_hash_addr. call thash_f_ll.
   auto => /> * ; do split ; smt(@W32).
-- admit. (* TODO: dont replace memcpyu8u8p *)
+- inline Mp(Syscall)._x_memcpy_u8u8p_32 Mp(Syscall)._memcpy_u8u8p_32. wp.
+  call memcpy_ptr_32_ll. auto => />. progress ; [ rewrite to_uintD_small /# | smt(@W64) ].
 qed.
 
-(* Chain Lengths *)
 lemma chain_lengths_ll : islossless Mp(Syscall).__chain_lengths.
 proof.
-proc.
-auto => /> ; call (checksum_ll).
-auto => /> ; call (base_w_ll).
-auto => />.
+proc ; wp.
+call checksum_ll ; wp.
+call base_w_ll ; wp.
+skip => /> *.
 by rewrite /to_list size_mkseq.
 qed.
 
@@ -151,7 +232,6 @@ while (#pre /\ 0 <= to_uint i <= size in_0) ((size in_0) - (to_uint i)) ; auto =
   - progress ; [ apply size_ge0 | smt(@W64) ].
 qed.
 
-(* Expand Seed *)
 lemma expand_seed_ll : islossless Mp(Syscall).__expand_seed.
 proof.
 proc.
@@ -173,13 +253,13 @@ while (true) (67 - i).
     call expand_seed_ll ; by auto => /> /#.
 qed.
 
-(* Sign *)
 lemma wots_sign_ll : islossless Mp(Syscall).__wots_sign.
 proof.
 proc.
 sp ; wp.
 while (true) (67 - i).
-- auto => />. inline Mp(Syscall).__set_chain_addr ; call gen_chain_inplace_ll ; auto => /> *. do split.
+- auto => />. inline Mp(Syscall).__set_chain_addr ; call gen_chain_inplace_ll ; auto => /> *. 
+  rewrite /XMSS_WOTS_W ; do split.
   + smt(@Array67 @W32).
   + admit.
   + admit.
@@ -194,18 +274,17 @@ proof.
 proc => //=.
 while (true) (67 - i).
 - auto => />. inline Mp(Syscall).__gen_chain_ ; inline Mp(Syscall)._gen_chain Mp(Syscall).__set_chain_addr ; auto => />.
-  call gen_chain_ll. auto => /> *. do split.
+  call gen_chain_ll. auto => /> *. rewrite /XMSS_WOTS_W //=. do split.
+  + smt(@Array67 @W32).
   + admit.
+  + smt (@Array67 @W32).
   + admit.
+  + smt (@Array67 @W32).
   + admit.
-  + admit.
-  + admit.
-  + admit.
-  + admit.
+  + progress => /#.
 - inline Mp(Syscall).__chain_lengths_ ; inline Mp(Syscall)._chain_lengths ; auto => />.
   call chain_lengths_ll ; by auto => /> /#.
 qed.
-
 
 (* XMSS *)
 
@@ -221,11 +300,10 @@ inline Mp(Syscall).__cond_u64_geq_u64_u32_eq_u32. wp.
 while (0 <= j <= 32) (32 - j).
 - admit.
 - auto => />; first by progress ; 1,3:smt(@W32) ; smt(). do call zero_addr_ll.
-  skip ; progress. 
+  skip => /> * ; do split.
   + admit.
   + admit.
-  + rewrite ultE of_uintK. admit. (* bounds on idx *)
-  + smt().
+  + move => *. split ; last by smt(). rewrite ultE. move => ???. rewrite of_uintK. admit. (* TODO: no info about idx *)
 qed.
 
 lemma gen_leaf_ll : islossless Mp(Syscall).__gen_leaf_wots.
@@ -251,11 +329,15 @@ while (0 <= to_uint i <= (10 - 1)) ((10 - 1) - (to_uint  i)).
     * rewrite to_uintD_small /#.
     * smt(@W64).
     * rewrite to_uintD_small ; smt(@W64).
-- wp ; sp. if ; last by admit.
-  +  inline Mp(Syscall)._x_memcpy_u8u8p_32 Mp(Syscall)._memcpy_u8u8p_32 ;wp ; call memcpy_ptr_32_ll.
-     wp. call memcpy_ll. skip => />. progress.
-    * by rewrite /to_list size_mkseq.
-    * smt(@W64).
+- wp ; sp. if.
+  + inline Mp(Syscall)._x_memcpy_u8u8p_32 Mp(Syscall)._memcpy_u8u8p_32 ;wp ; call memcpy_ptr_32_ll.
+    wp. call memcpy_ll. skip => />. progress.
+     * by rewrite /to_list size_mkseq.
+     * smt(@W64).
+  + inline Mp(Syscall)._x_memcpy_u8u8p_32 Mp(Syscall)._memcpy_u8u8p_32 ; wp ; call memcpy_ptr_32_ll. 
+    wp ; call memcpy_ll. skip => /> *. split.
+     * by rewrite /to_list size_mkseq.
+     * smt (@W64).
 qed.
 
 lemma keypair_seed_ll : islossless Mp(Syscall).__xmssmt_core_seed_keypair.
@@ -270,20 +352,69 @@ do (wp ; call memcpy_ll).
 wp. call memset_zero_ll.
 inline Mp(Syscall).__set_layer_addr.
 wp ; sp. call zero_addr_ll.
-skip ; progress; 1,2,3: by smt(@List @Array96 @Array64 @Array32).
-  + smt().
-  + smt().
+skip ; progress; by smt(@List @Array96 @Array64 @Array32).
 qed.
 
-lemma randombytes_ll : islossless Syscall.randombytes_96.
-proof.
-proc.
-admit.
-qed.
+lemma randombytes_ll : islossless Syscall.randombytes_96
+    by proc ; islossless ; smt.
 
 lemma keypair_ll : islossless Mp(Syscall).__xmssmt_core_keypair.
 proof.
 proc.
 call keypair_seed_ll ; call randombytes_ll.
 by auto.
+qed.
+
+lemma set_result_ll : phoare [Mp(Syscall).__set_result :
+      0 <= to_uint (loadW64 Glob.mem (to_uint mlen_ptr)) < W64.max_uint ==> true] = 1%r.
+proof.
+proc.
+if.
+- wp; call memset_u8_ptr_ll. auto => /> /#.
+- inline Mp(Syscall)._x__memcpy_u8pu8p Mp(Syscall)._memcpy_u8pu8p ; wp.
+  call memcpy_ptr_ptr_ll. wp ; skip => /> *.
+qed.
+
+lemma sign_open_ll : phoare [Mp(Syscall).__xmssmt_core_sign_open :
+    0 <= to_uint (loadW64 Glob.mem (to_uint mlen_ptr)) < W64.max_uint ==>
+    true] = 1%r.
+proof.
+proc.
+wp ; sp.
+inline Mp(Syscall).__set_type Mp(Syscall).__set_layer_addr  Mp(Syscall).__set_tree_addr Mp(Syscall).__set_ots_addr 
+       Mp(Syscall).__set_ltree_addr.
+sp ; wp.
+call set_result_ll. call memcmp_ll.
+while (0 <= to_uint i <= 1) (1 - to_uint i); auto => />.
+  + inline Mp(Syscall).__compute_root_ Mp(Syscall)._compute_root ; wp ; call compute_root_ll ; wp.
+    inline Mp(Syscall).__l_tree_ Mp(Syscall)._l_tree ; wp ; call ltree_ll ; wp.
+    inline Mp(Syscall).__wots_pk_from_sig_ ; wp ; call wots_pk_from_sig_ll ; wp. skip => /> * ; do split.
+    * rewrite to_uintD_small /#.
+    * smt(@W32).
+    * smt(@W32).
+  + progress ; smt(@W32). 
+  + call hash_msg_ll ; inline Mp(Syscall)._x_memcpy_u8u8p_32 Mp(Syscall)._memcpy_u8u8p_32 ; wp.
+    call memcpy_ptr_32_ll ; wp. inline Mp(Syscall)._x__memcpy_u8pu8p Mp(Syscall)._memcpy_u8pu8p ; wp. 
+    call memcpy_ptr_ptr_ll ; wp. call bytes_to_ull_ptr_ll ; wp. do 3! call zero_addr_ll. 
+    skip => /> *. progress.
+    * smt(@W32).
+    * smt.
+    * admit.
+qed.
+
+lemma sign_ll : islossless Mp(Syscall).__xmssmt_core_sign.
+proof.
+proc.
+wp ; sp.
+admit.
+qed.
+
+
+
+(******************************* exported functions **********************************)
+lemma kg_ll : islossless Mp(Syscall).xmss_keypair_jazz.
+proof.
+proc.
+inline Mp(Syscall).__xmss_keypair Mp(Syscall).__xmssmt_core_keypair_ Mp(Syscall)._xmssmt_core_keypair.
+wp ; sp. call keypair_ll. by skip.
 qed.
